isabelle/Chapter16_2_Expression.thy
@@ -69,8 +69,8 @@ where "subst' n e' (Var v) = (if v = n then e' else Var v)"
     | "subst' n e' (Fold t e) = Fold t (subst' n e' e)"
     | "subst' n e' (Unfold e) = Unfold (subst' n e' e)"
 
-definition subst :: "expr => expr => expr"
-where "subst e' e = remove first (subst' first (insert first e') e)"
+definition subst :: "expr => var => expr => expr"
+where "subst e' n e = remove first (subst' first (insert first e') e)"
 
 lemma [simp]: "remove n (insert n e) = e"
 by (induction e arbitrary: n, simp_all)
@@ -81,7 +81,7 @@ by (induction e arbitrary: n m, simp_all)
 lemma [simp]: "remove v (subst' v (insert v e') (insert v e)) = e"
 by (induction e arbitrary: e' v, simp_all)
 
-lemma [simp]: "subst e' (insert first e) = e"
+lemma [simp]: "subst e' first (insert first e) = e"
 by (simp add: subst_def)
 
 end
