isabelle/Chapter09_3_Evaluation.thy
@@ -15,10 +15,10 @@ where eval_suc [simp]: "eval e e' ==> eval (Suc e) (Suc e')"
     | eval_rec_1 [simp]: "eval et et' ==> eval (Rec et e0 es) (Rec et' e0 es)"
     | eval_rec_2 [simp]: "eval (Rec Zero e0 es) e0"
     | eval_rec_3 [simp]: "is_val et ==> 
-            eval (Rec (Suc et) e0 es) (subst (Rec et e0 es) (subst et es))"
+            eval (Rec (Suc et) e0 es) (subst (Rec et e0 es) first (subst et first es))"
     | eval_appl_1 [simp]: "eval e1 e1' ==> eval (Appl e1 e2) (Appl e1' e2)"
     | eval_appl_2 [simp]: "is_val e1 ==> eval e2 e2' ==> eval (Appl e1 e2) (Appl e1 e2')"
-    | eval_appl_3 [simp]: "is_val e2 ==> eval (Appl (Lam t2 e1) e2) (subst e2 e1)"
+    | eval_appl_3 [simp]: "is_val e2 ==> eval (Appl (Lam t2 e1) e2) (subst e2 first e1)"
 
 lemma canonical_nat: "is_val e ==> typecheck gam e Nat ==> 
           e = Zero | (EX e'. e = Suc e' & typecheck gam e' Nat)"
@@ -40,7 +40,7 @@ next case eval_rec_1
 next case eval_rec_2 
   thus ?case by fastforce
 next case (eval_rec_3 et e0 es)
-  from eval_rec_3 canonical_nat_no_vars have "typecheck (extend gam t) (subst et es) t" by auto
+  from eval_rec_3 canonical_nat_no_vars have "typecheck (extend gam t) (subst et first es) t" by auto
   with eval_rec_3 show ?case by fastforce
 next case eval_appl_1 
   thus ?case by fastforce
