isabelle/Chapter12_4_Evaluation.thy
@@ -26,10 +26,10 @@ where eval_suc [simp]: "eval e e' ==> eval (Suc e) (Suc e')"
     | eval_rec_1 [simp]: "eval et et' ==> eval (Rec et e0 es) (Rec et' e0 es)"
     | eval_rec_2 [simp]: "eval (Rec Zero e0 es) e0"
     | eval_rec_3 [simp]: "is_val et ==> 
-            eval (Rec (Suc et) e0 es) (subst (Rec et e0 es) (subst et es))"
+            eval (Rec (Suc et) e0 es) (subst (Rec et e0 es) first (subst et first es))"
     | eval_appl_1 [simp]: "eval e1 e1' ==> eval (Appl e1 e2) (Appl e1' e2)"
     | eval_appl_2 [simp]: "is_val e1 ==> eval e2 e2' ==> eval (Appl e1 e2) (Appl e1 e2')"
-    | eval_appl_3 [simp]: "is_val e2 ==> eval (Appl (Lam t2 e1) e2) (subst e2 e1)"
+    | eval_appl_3 [simp]: "is_val e2 ==> eval (Appl (Lam t2 e1) e2) (subst e2 first e1)"
     | eval_pair_1 [simp]: "eval e1 e1' ==> eval (Pair e1 e2) (Pair e1' e2)"
     | eval_pair_2 [simp]: "is_val e1 ==> eval e2 e2' ==> eval (Pair e1 e2) (Pair e1 e2')"
     | eval_projl_1 [simp]: "eval e e' ==> eval (ProjL e) (ProjL e')"
@@ -38,8 +38,8 @@ where eval_suc [simp]: "eval e e' ==> eval (Suc e) (Suc e')"
     | eval_projr_2 [simp]: "eval (ProjR (Pair e1 e2)) e2"
     | eval_abort [simp]: "eval e e' ==> eval (Abort t e) (Abort t e')"
     | eval_case_1 [simp]: "eval et et' ==> eval (Case et el er) (Case et' el er)"
-    | eval_case_2 [simp]: "is_val e ==> eval (Case (InL t1 t2 e) el er) (subst e el)"
-    | eval_case_3 [simp]: "is_val e ==> eval (Case (InR t1 t2 e) el er) (subst e er)"
+    | eval_case_2 [simp]: "is_val e ==> eval (Case (InL t1 t2 e) el er) (subst e first el)"
+    | eval_case_3 [simp]: "is_val e ==> eval (Case (InR t1 t2 e) el er) (subst e first er)"
     | eval_inl [simp]: "eval e e' ==> eval (InL t1 t2 e) (InL t1 t2 e')"
     | eval_inr [simp]: "eval e e' ==> eval (InR t1 t2 e) (InR t1 t2 e')"
     | eval_match_1 [simp]: "eval e e' ==> eval (Match e rs) (Match e' rs)"
@@ -124,7 +124,7 @@ next case eval_rec_1
 next case eval_rec_2 
   thus ?case by fastforce
 next case (eval_rec_3 et e0 es)
-  from eval_rec_3 canonical_nat_no_vars have "typecheck (extend gam t) (subst et es) t" by auto
+  from eval_rec_3 canonical_nat_no_vars have "typecheck (extend gam t) (subst et first es) t" by auto
   with eval_rec_3 show ?case by fastforce
 next case eval_appl_1 
   thus ?case by fastforce
